Splitting the file of the definition of the logical relation and replacing type reducibility with type reducible conversion

theories/GenericTyping.v
@@ -34,18 +34,6 @@ Section RedDefinitions.
 
   (** *** Bundling of a predicate with side-conditions *)
 
-  Record TypeRedWhnf (Γ : context) (A B : term) : Type :=
-    {
-      tyred_whnf_red :> [ Γ |- A ⤳* B ] ;
-      tyred_whnf_whnf :> whnf B
-    }.
-
-  Record TermRedWhnf (Γ : context) (A t u : term) : Type :=
-    {
-      tmred_whnf_red :> [ Γ |- t ⤳* u : A ] ;
-      tmred_whnf_whnf :> whnf u
-    }.
-
   Record TypeConvWf (Γ : context) (A B : term) : Type :=
     {
       tyc_wf_l : [Γ |- A] ;
@@ -60,15 +48,30 @@ Section RedDefinitions.
       tmc_wf_conv :> [Γ |- t ≅ u : A]
     }.
 
-  Record TypeRedWf (Γ : context) (A B : term) : Type := {
+  Record TypeRedWf {Γ : context} {A B : term} : Type := {
     tyr_wf_r : [Γ |- B];
     tyr_wf_red :> [Γ |- A ⤳* B]
   }.
 
-  Record TermRedWf (Γ : context) (A t u : term) : Type := {
+  Record TermRedWf {Γ : context} {A t u : term} : Type := {
     tmr_wf_r : [Γ |- u : A];
     tmr_wf_red :> [Γ |- t ⤳* u : A]
   }.
+
+  Record TypeRedWhnf {Γ : context} {A : term} : Type :=
+    {
+      tyred_whnf : term ;
+      tyred_whnf_red :> @TypeRedWf Γ A tyred_whnf ;
+      tyred_whnf_isType :> isType tyred_whnf
+    }.
+
+
+  Record TermRedWhnf {Γ : context} {A t : term} : Type :=
+    {
+      tmred_whnf : term ;
+      tmred_whnf_red :> @TermRedWf Γ A t tmred_whnf ;
+      tmred_whnf_whnf :> whnf tmred_whnf
+    }.
 
   (** *** Lifting of typing and conversion to contexts and substitutions *)
 
@@ -147,10 +150,20 @@ Section RedDefinitions.
 
 End RedDefinitions.
 
-Notation "[ Γ |- A ↘ B ]" := (TypeRedWhnf Γ A B) (only parsing) : typing_scope.
-Notation "[ Γ |-[ ta  ] A ↘ B ]" := (TypeRedWhnf (ta := ta) Γ A B) : typing_scope.
-Notation "[ Γ |- t ↘ u : A ]" := (TermRedWhnf Γ A t u) (only parsing ): typing_scope.
-Notation "[ Γ |-[ ta  ] t ↘ u : A ]" := (TermRedWhnf (ta := ta) Γ A t u) : typing_scope.
+Arguments TypeRedWf : clear implicits.
+Arguments TypeRedWf {_ _ _}.
+Arguments TermRedWf : clear implicits.
+Arguments TermRedWf {_ _ _}.
+Arguments TypeRedWhnf : clear implicits.
+Arguments TypeRedWhnf {_ _ _}.
+Arguments TermRedWhnf : clear implicits.
+Arguments TermRedWhnf {_ _ _}.
+
+
+Notation "[ Γ |- A ↘ ]" := (TypeRedWhnf Γ A) (only parsing) : typing_scope.
+Notation "[ Γ |-[ ta  ] A ↘ ]" := (TypeRedWhnf (ta := ta) Γ A) : typing_scope.
+Notation "[ Γ |- t ↘ A ]" := (TermRedWhnf Γ A t) (only parsing ): typing_scope.
+Notation "[ Γ |-[ ta  ] t ↘ A ]" := (TermRedWhnf (ta := ta) Γ A t) : typing_scope.
 Notation "[ Γ |- A :≅: B ]" := (TypeConvWf Γ A B) (only parsing) : typing_scope.
 Notation "[ Γ |-[ ta  ] A :≅: B ]" := (TypeConvWf (ta := ta) Γ A B) : typing_scope.
 Notation "[ Γ |- t :≅: u : A ]" := (TermConvWf Γ A t u) (only parsing) : typing_scope.
@@ -172,6 +185,10 @@ Notation "[ |-[ ta  ] Γ ≅ Δ ]" := (ConvCtx (ta := ta) Γ Δ) : typing_scope.
   well_sempty well_scons conv_sempty conv_scons
   tyr_wf_r tyr_wf_red tmr_wf_r tmr_wf_red
   : gen_typing.
+
+#[export] Hint Extern 1 =>
+  now unshelve first [ eapply tyred_whnf_red|eapply tmred_whnf_red
+    | eapply tyred_whnf_isType| eapply tmred_whnf_whnf] : gen_typing.
 
 (* #[export] Hint Extern 1 =>
   match goal with
@@ -820,6 +837,30 @@ Section GenericConsequences.
     intros ??? [] []; unshelve econstructor; try etransitivity; tea.
   Qed.
 
+  Definition convty_wfexp {Γ A A' B B'} :
+    [Γ |- A :⤳*: A'] ->
+    [Γ |- B :⤳*: B'] ->
+    [Γ |- A' ≅ B'] ->
+    [Γ |- A ≅ B].
+  Proof.
+    intros; eapply convty_exp; gtyping.
+  Qed.
+
+  Definition convtm_wfexp {Γ A A' t t' u u'} :
+    [Γ |- A :⤳*: A'] ->
+    [Γ |- t :⤳*: t' : A'] ->
+    [Γ |- u :⤳*: u' : A'] ->
+    [Γ |- t' ≅ u' : A'] ->
+    [Γ |- A' ≅ A'] ->
+    [Γ |- t ≅ u : A].
+  Proof.
+    intros.
+    assert [Γ |- A' ≅ A] by (eapply convty_wfexp; tea; gtyping).
+    eapply convtm_conv; tea.
+    eapply convtm_exp; tea; gtyping.
+  Qed.
+
+
   Lemma redtmwf_app {Γ A B f f' t} :
     [ Γ |- f :⤳*: f' : tProd A B ] ->
     [ Γ |- t : A ] ->
@@ -1275,23 +1316,19 @@ Section GenericConsequences.
     all: now eapply redty_sound.
   Qed.
 
-  (* Unused, consider removing*)
-  Lemma whredtm_det Γ t u u' A A' :
-    [Γ |- t ↘ u : A] -> [Γ |- t ↘ u' : A'] ->
-    u = u'.
+  Lemma whredtm_det Γ t A A' (red1 : [Γ |- t ↘ A]) (red2 : [Γ |- t ↘ A']) :
+    red1.(tmred_whnf) = red2.(tmred_whnf).
   Proof.
-    intros [] [].
+    destruct red1 as [? []], red2 as [? []]; cbn.
     eapply whred_det; tea.
     all: now eapply redtm_sound.
   Qed.
 
-  (* Unused, consider removing*)
-  Lemma whredty_det Γ A B B' :
-    [Γ |- A ↘ B] -> [Γ |- A ↘ B'] ->
-    B = B'.
+  Lemma whredty_det Γ A (red1 : [Γ |- A ↘]) (red2 : [Γ |- A ↘]) :
+   red1.(tyred_whnf) = red2.(tyred_whnf).
   Proof.
-    intros [] [].
-    eapply whred_det; tea.
+    destruct red1 as [? []], red2 as [? []]; cbn.
+    eapply whred_det; try eapply isType_whnf; tea.
     all: now eapply redty_sound.
   Qed.
 
