theories/LogicalRelation/Definition/Helper.v
@@ -1,0 +1,356 @@
+(** * LogRel.LogicalRelation.Definition.Helper: Auxilliary definitions and rebundling of structures from the logical relation *)
+From Coq Require Import CRelationClasses.
+From LogRel Require Import Utils Syntax.All GenericTyping.
+From LogRel.LogicalRelation.Definition Require Import Prelude Ne Universe Poly Pi Sig Nat Empty Id Def.
+
+Set Primitive Projections.
+Set Universe Polymorphism.
+Set Polymorphic Inductive Cumulativity.
+
+Lemma instKripke `{GenericTypingProperties} {Γ A B l} (wfΓ : [|-Γ])
+  (h : forall Δ (ρ : Δ ≤ Γ) (wfΔ : [|-Δ]), [Δ ||-<l> A⟨ρ⟩ ≅ B⟨ρ⟩]) : [Γ ||-<l> A ≅ B].
+Proof.
+  specialize (h Γ wk_id wfΓ); now rewrite 2!wk_id_ren_on in h.
+Qed.
+
+
+(** ** Rebundling reducibility of Polynomial *)
+
+(** The definition of reducibility of product types in the logical relation, which separates
+the "adequacy" part is not nice to work with. Here we relate it to the more natural one,
+which lets us later on define an induction principle that does not show the separation at all. *)
+
+Module PolyRed.
+
+Section PolyRed.
+  Context `{ta : tag}
+    `{!WfContext ta} `{!WfType ta} `{!Typing ta}
+    `{!ConvType ta} `{!ConvTerm ta} `{!ConvNeuConv ta}
+    `{!RedType ta} `{!RedTerm ta}
+    {Γ : context} {l : TypeLevel} {shp shp' pos pos' : term}.
+
+  Record PolyRed@{i j k l} : Type@{l} :=
+    {
+      shpRed [Δ] (ρ : Δ ≤ Γ) : [ |- Δ ] -> [ LogRel@{i j k l} l | Δ ||- shp⟨ρ⟩ ≅ shp'⟨ρ⟩ ] ;
+      posRed [Δ a b] (ρ : Δ ≤ Γ) (h : [ |- Δ ]) :
+          [ (shpRed ρ h) |  Δ ||- a ≅ b : shp⟨ρ⟩] ->
+          [ LogRel@{i j k l} l | Δ ||- pos[a .: (ρ >> tRel)] ≅ pos'[b .: (ρ >> tRel)]] ;
+      (* posExt
+        [Δ a b]
+        (ρ : Δ ≤ Γ)
+        (h :  [ |- Δ ])
+        (hab : [ (shpRed ρ h) | Δ ||- a ≅ b : shp⟨ρ⟩]) :
+        [ (posRed ρ h hab) | Δ ||- (pos[a .: (ρ >> tRel)]) ≅ (pos[b .: (ρ >> tRel)]) ] *)
+    }.
+
+  Definition from@{i j k l} {PA : PolyRedPack@{k} Γ shp shp' pos pos'}
+    (PAad : PolyRedPackAdequate@{k l} (LogRel@{i j k l} l) PA)
+    : PolyRed@{i j k l}.
+  Proof.
+    unshelve econstructor; intros.
+    - econstructor; unshelve eapply PolyRedPack.shpAd; cycle 2; tea.
+    - econstructor; unshelve eapply PolyRedPack.posAd; cycle 2; tea.
+  Defined.
+
+  Definition toPack@{i j k l} (PA : PolyRed@{i j k l}) : PolyRedPack@{k} Γ shp shp' pos pos'.
+  Proof.
+    unshelve econstructor.
+    - now eapply shpRed.
+    - intros; now eapply posRed.
+  Defined.
+
+  Definition toAd@{i j k l} (PA : PolyRed@{i j k l}) : PolyRedPackAdequate@{k l} (LogRel@{i j k l} l) (toPack PA).
+  Proof.
+    unshelve econstructor; intros.
+    - eapply LRAd.adequate; eapply posRed.
+    - eapply LRAd.adequate; eapply shpRed.
+  Defined.
+
+  Lemma eta@{i j k l} (PA : PolyRed@{i j k l}) : from (toAd PA) = PA.
+  Proof. destruct PA; reflexivity. Qed.
+
+  Lemma beta_pack@{i j k l} {PA : PolyRedPack@{k} Γ shp shp' pos pos'}
+    (PAad : PolyRedPackAdequate@{k l} (LogRel@{i j k l} l) PA)
+    : toPack (from PAad) = PA.
+  Proof. destruct PA, PAad; reflexivity. Qed.
+
+  Lemma beta_ad@{i j k l} {PA : PolyRedPack@{k} Γ shp shp' pos pos'}
+    (PAad : PolyRedPackAdequate@{k l} (LogRel@{i j k l} l) PA)
+    : toAd (from PAad) = PAad.
+  Proof. destruct PA, PAad; reflexivity. Qed.
+
+End PolyRed.
+
+Arguments PolyRed : clear implicits.
+Arguments PolyRed {_ _ _ _ _ _ _ _ _} _ _ _ _ _.
+
+End PolyRed.
+
+Export PolyRed(PolyRed,Build_PolyRed).
+Coercion PolyRed.toPack : PolyRed >-> PolyRedPack.
+
+Module ParamRedTy.
+Section ParamRedTy.
+  Context {T : term -> term -> term} `{ta : tag}
+    `{!WfContext ta} `{!WfType ta} `{!Typing ta}
+    `{!ConvType ta} `{!ConvTerm ta} `{!ConvNeuConv ta}
+    `{!RedType ta} `{!RedTerm ta}
+    {Γ : context} {l : TypeLevel} {A B : term}.
+
+  Record ParamRedTy@{i j k l} : Type@{l} :=
+    {
+      domL : term ;
+      domR : term ;
+      codL : term ;
+      codR : term ;
+      redL : ParamRedTyPack.ParamTy (T:=T) Γ A domL codL ;
+      redR : ParamRedTyPack.ParamTy (T:=T) Γ B domR codR ;
+      eqdom : [Γ |- domL ≅ domR];
+      eq : [Γ |- T domL codL ≅ T domR codR] ;
+      polyRed :> PolyRed@{i j k l} Γ l domL domR codL codR
+    }.
+
+  Definition from@{i j k l} {PA : ParamRedTyPack@{k} (T:=T) Γ A B}
+    (PAad : PolyRedPackAdequate@{k l} (LogRel@{i j k l} l) PA) :
+    ParamRedTy@{i j k l}.
+  Proof.
+    exists (ParamRedTyPack.domL PA) (ParamRedTyPack.domR PA)
+      (ParamRedTyPack.codL PA) (ParamRedTyPack.codR PA).
+    - eapply ParamRedTyPack.redL.
+    - eapply ParamRedTyPack.redR.
+    - eapply ParamRedTyPack.eqdom.
+    - eapply ParamRedTyPack.eq.
+    - now eapply PolyRed.from.
+  Defined.
+
+  Definition toPack@{i j k l} (PA : ParamRedTy@{i j k l}) :
+    ParamRedTyPack@{k} (T:=T) Γ A B.
+  Proof.
+    exists (domL PA) (domR PA) (codL PA) (codR PA).
+    - now eapply redL.
+    - now eapply redR.
+    - apply eqdom.
+    - now eapply eq.
+    - exact (PolyRed.toPack PA).
+  Defined.
+
+  Definition toAd@{i j k l} (PA : ParamRedTy@{i j k l}) :
+    PolyRedPackAdequate@{k l} (LogRel@{i j k l} l) (toPack PA) :=
+    PolyRed.toAd PA.
+
+  Lemma eta@{i j k l} (PA : ParamRedTy@{i j k l}) : from (toAd PA) = PA.
+  Proof. destruct PA; reflexivity. Qed.
+
+  Lemma beta_pack@{i j k l} {PA : ParamRedTyPack@{k} (T:=T) Γ A B}
+    (PAad : PolyRedPackAdequate@{k l} (LogRel@{i j k l} l) PA)
+    : toPack (from PAad) = PA.
+  Proof. destruct PA, PAad; reflexivity. Qed.
+
+  Lemma beta_ad@{i j k l} {PA : ParamRedTyPack@{k} (T:=T) Γ A B}
+    (PAad : PolyRedPackAdequate@{k l} (LogRel@{i j k l} l) PA)
+    : toAd (from PAad) = PAad.
+  Proof. destruct PA, PAad; reflexivity. Qed.
+End ParamRedTy.
+
+Arguments ParamRedTy : clear implicits.
+Arguments ParamRedTy _ {_ _ _ _ _ _ _ _ _}.
+
+End ParamRedTy.
+
+(** ** Rebundling reducibility of product and sigma types *)
+
+Export ParamRedTy(ParamRedTy, Build_ParamRedTy).
+Coercion ParamRedTy.polyRed : ParamRedTy >-> PolyRed.
+Coercion ParamRedTy.toPack : ParamRedTy >-> ParamRedTyPack.
+
+Section EvenMoreDefs.
+  Context `{ta : tag}
+    `{!WfContext ta} `{!WfType ta} `{!Typing ta}
+    `{!ConvType ta} `{!ConvTerm ta} `{!ConvNeuConv ta}
+    `{!RedType ta} `{!RedTerm ta}.
+
+  Definition PiRedTy@{i j k l} Γ l A B := ParamRedTy@{i j k l} tProd Γ l A B.
+  Definition SigRedTy@{i j k l} Γ l A B := ParamRedTy@{i j k l} tSig Γ l A B.
+
+  Definition LRPi'@{i j k l} {l Γ A B} (ΠA : PiRedTy@{i j k l} Γ l A B)
+    : [ LogRel@{i j k l} l | Γ ||- A ≅ B ] :=
+    LRbuild (LRPi (LogRelRec l) _ (ParamRedTy.toAd ΠA)).
+
+  Definition LRSig' @{i j k l} {l Γ A B} (ΠA : SigRedTy@{i j k l} Γ l A B)
+    : [ LogRel@{i j k l} l | Γ ||- A ≅ B] :=
+    LRbuild (LRSig (LogRelRec l) _ (ParamRedTy.toAd ΠA)).
+
+End EvenMoreDefs.
+
+Notation "[ Γ ||-Π< l > A ≅ B ]" := (PiRedTy Γ l A B) (at level 0, Γ, l, A, B at level 50).
+Notation "[ Γ ||-Σ< l > A ≅ B ]" := (SigRedTy Γ l A B) (at level 0, Γ, l, A, B at level 50).
+Notation "[ Γ ||-Π t ≅ u : A | ΠA ]" := (PiRedTmEq (Γ:=Γ) (A:=A) t u (ParamRedTy.toPack ΠA)).
+Notation "[ Γ ||-Σ t ≅ u : A | ΣA ]" := (SigRedTmEq (Γ:=Γ) (A:=A) t u (ParamRedTy.toPack ΣA)).
+
+Module PiRedTy.
+  Include ParamRedTyPack.
+
+  Section PiRedTy.
+  Context `{GenericTypingProperties}.
+  Definition whredL  {l Γ A B} : PiRedTy Γ l A B -> [Γ |- A ↘ ] :=
+    ParamRedTyPack.whredL0 (T:=tProd) ltac:(intros; constructor).
+  Definition whredR  {l Γ A B} : PiRedTy Γ l A B -> [Γ |- B ↘ ] :=
+    ParamRedTyPack.whredR0 (T:=tProd) ltac:(intros; constructor).
+  End PiRedTy.
+End PiRedTy.
+
+Module SigRedTy.
+  Include ParamRedTyPack.
+
+  Section SigRedTy.
+  Context `{GenericTypingProperties}.
+  Definition whredL  {l Γ A B} : SigRedTy Γ l A B -> [Γ |- A ↘ ] :=
+    ParamRedTyPack.whredL0 (T:=tSig) ltac:(intros; constructor).
+  Definition whredR  {l Γ A B} : SigRedTy Γ l A B -> [Γ |- B ↘ ] :=
+    ParamRedTyPack.whredR0 (T:=tSig) ltac:(intros; constructor).
+  End SigRedTy.
+End SigRedTy.
+
+
+
+
+(* * ** Properties of reducibility at Nat and Empty
+
+Lemma NatPropEq_whnf `{GenericTypingProperties} {Γ A t u} {NA : [Γ ||-Nat A]} : NatPropEq NA t u -> whnf t × whnf u.
+Proof.  intros [ | | ? ? []]; split; econstructor; eapply convneu_whne; first [eassumption|symmetry; eassumption]. Qed.
+
+Lemma EmptyPropEq_whnf `{GenericTypingProperties} {Γ A t u} {NA : [Γ ||-Empty A]} : EmptyPropEq Γ t u -> whnf t × whnf u.
+Proof.  intros [ ? ? []]; split; econstructor; eapply convneu_whne; first [eassumption|symmetry; eassumption]. Qed.
+
+(* A&Y: We prove the hand-crafted induction principles here: *)
+
+Lemma EmptyRedEqInduction :
+  forall {ta : tag} {H0 : WfType ta} {H2 : RedType ta} {H3 : Typing ta}
+    {H4 : ConvNeuConv ta} {H5 : ConvTerm ta} {H6 : RedTerm ta}
+    (Γ : context) (A : term) (NA : [Γ ||-Empty A])
+    (P : forall t t0 : term, [Γ ||-Empty t ≅ t0 : A | NA] -> Type)
+    (P0 : forall t t0 : term, EmptyPropEq Γ t t0 -> Type),
+    (forall (t u nfL nfR : term) (redL : [Γ |-[ ta ] t :⤳*: nfL : tEmpty])
+       (redR : [Γ |-[ ta ] u :⤳*: nfR : tEmpty]) (eq : [Γ |-[ ta ] nfL ≅ nfR : tEmpty])
+       (prop : EmptyPropEq Γ nfL nfR),
+        P0 nfL nfR prop -> P t u (Build_EmptyRedTmEq nfL nfR redL redR eq prop)) ->
+    (forall (ne ne' : term) (r : [Γ ||-NeNf ne ≅ ne' : tEmpty]),
+        P0 ne ne' (EmptyRedTmEq.neReq r)) ->
+    (forall (t t0 : term) (n : [Γ ||-Empty t ≅ t0 : A | NA]), P t t0 n)
+      × (forall (t t0 : term) (n : EmptyPropEq Γ t t0), P0 t t0 n).
+Proof.
+  intros.
+  split.
+  - intros t t0 n. induction n.
+    eapply X; eauto. destruct prop; eauto.
+  - intros. induction n. eapply X0.
+Qed. *)
+
+Module IdRedTy.
+Section IdRedTy.
+
+  Context `{ta : tag}
+    `{!WfContext ta} `{!WfType ta} `{!Typing ta}
+    `{!ConvType ta} `{!ConvTerm ta} `{!ConvNeuConv ta}
+    `{!RedType ta} `{!RedTerm ta}.
+
+  Record IdRedTy@{i j k l} {Γ : context} {l} {A B : term}
+  : Type :=
+  {
+    tyL : term ;
+    tyR : term ;
+    lhsL : term ;
+    lhsR : term ;
+    rhsL : term ;
+    rhsR : term ;
+    redL : [Γ |- A :⤳*: tId tyL lhsL rhsL] ;
+    redR : [Γ |- B :⤳*: tId tyR lhsR rhsR] ;
+    eq : [Γ |- tId tyL lhsL rhsL ≅ tId tyR lhsR rhsR] ;
+    tyRed : [ LogRel@{i j k l} l | Γ ||- tyL ≅ tyR ] ;
+    lhsRed : [ tyRed | Γ ||- lhsL ≅ lhsR : _ ] ;
+    rhsRed : [ tyRed | Γ ||- rhsL ≅ rhsR : _ ] ;
+    (* Bake in PER property for reducible conversion at ty  to cut dependency cycles *)
+    tyPER : PER tyRed.(LRPack.eqTm) ;
+    tyKripke : forall {Δ} (ρ : Δ ≤ Γ) (wfΔ : [|-Δ]), [LogRel@{i j k l} l| Δ ||- tyL⟨ρ⟩ ≅ tyR⟨ρ⟩ ] ;
+    tyKripkeTmEq : forall {Δ Ξ} (ρ : Δ ≤ Γ) (ρ' : Ξ ≤ Γ) (ρ'' : Ξ ≤ Δ) (wfΔ : [|-Δ]) (wfΞ : [|-Ξ]) t u,
+      ρ' =1 ρ'' ∘w ρ -> [tyKripke ρ wfΔ | _ ||- t ≅ u : _] -> [tyKripke ρ' wfΞ | _ ||- t⟨ρ''⟩ ≅ u⟨ρ''⟩ : _];
+  }.
+
+
+
+  Definition from@{i j k l} {Γ l A B} {IA : IdRedTyPack@{k} Γ A B} (IAad : IdRedTyAdequate@{k l} (LogRel@{i j k l} l) IA)
+    : @IdRedTy@{i j k l} Γ l A B.
+  Proof.
+    unshelve econstructor; try (exact IA.(IdRedTyPack.redL) + exact IA.(IdRedTyPack.redR)).
+    - econstructor; apply IAad.
+    - intros; econstructor; (unshelve now eapply IAad); tea.
+    - exact IA.(IdRedTyPack.eq).
+    - exact IA.(IdRedTyPack.lhsRed).
+    - exact IA.(IdRedTyPack.rhsRed).
+    - exact IA.(IdRedTyPack.tyPER).
+    - intros; now eapply IA.(IdRedTyPack.tyKripkeTmEq).
+  Defined.
+
+  Definition toPack@{i j k l} {Γ l A B} (IA : @IdRedTy@{i j k l} Γ l A B) : IdRedTyPack@{k} Γ A B.
+  Proof.
+    unshelve econstructor; try (exact IA.(IdRedTy.redL) + exact IA.(IdRedTy.redR)).
+    - apply IA.(tyRed).
+    - intros; now apply IA.(tyKripke).
+    - exact IA.(eq).
+    - exact IA.(lhsRed).
+    - exact IA.(rhsRed).
+    - exact IA.(IdRedTy.tyPER).
+    - intros; now eapply IA.(IdRedTy.tyKripkeTmEq).
+  Defined.
+
+  Definition to@{i j k l} {Γ l A B} (IA : @IdRedTy@{i j k l} Γ l A B) : IdRedTyAdequate@{k l} (LogRel@{i j k l} l) (toPack IA).
+  Proof.
+    econstructor; [apply IA.(tyRed)| intros; apply IA.(tyKripke)].
+  Defined.
+
+  Lemma beta_pack@{i j k l} {Γ l A B} {IA : IdRedTyPack@{k} Γ A B} (IAad : IdRedTyAdequate@{k l} (LogRel@{i j k l} l) IA) :
+    toPack (from IAad) = IA.
+  Proof. reflexivity. Qed.
+
+  Lemma beta_ad@{i j k l} {Γ l A B} {IA : IdRedTyPack@{k} Γ A B} (IAad : IdRedTyAdequate@{k l} (LogRel@{i j k l} l) IA) :
+    to (from IAad) = IAad.
+  Proof. reflexivity. Qed.
+
+  Lemma eta@{i j k l} {Γ l A B} (IA : @IdRedTy@{i j k l} Γ l A B) : from  (to IA) = IA.
+  Proof. reflexivity. Qed.
+
+  Definition IdRedTmEq {Γ l A B} (IA : @IdRedTy Γ l A B) := IdRedTmEq (toPack IA).
+  Definition IdPropEq {Γ l A B} (IA : @IdRedTy Γ l A B) := IdPropEq (toPack IA).
+
+  Definition LRId'@{i j k l} {l Γ A B} (IA : @IdRedTy@{i j k l} Γ l A B)
+    : [ LogRel@{i j k l} l | Γ ||- A ≅ B] :=
+    LRbuild (LRId (LogRelRec l) _ (to IA)).
+End IdRedTy.
+
+Arguments IdRedTy {_ _ _ _ _ _ _ _ _}.
+
+  Definition whredL `{GenericTypingProperties} {l Γ A B} : IdRedTy Γ l A B -> [Γ |- A ↘ ].
+  Proof. intros []; econstructor; tea; constructor. Defined.
+
+  Definition whredR `{GenericTypingProperties} {l Γ A B} : IdRedTy Γ l A B -> [Γ |- B ↘ ].
+  Proof. intros []; econstructor; tea; constructor. Defined.
+
+  Definition outTy `{GenericTypingProperties} {l Γ A B} (IA : IdRedTy Γ l A B) := IdRedTyPack.outTy (toPack IA).
+
+End IdRedTy.
+
+Export IdRedTy(IdRedTy, Build_IdRedTy,IdRedTmEq,IdPropEq,LRId').
+
+Notation "[ Γ ||-Id< l > A ≅ B ]" := (IdRedTy Γ l A B) (at level 0, Γ, l,  A, B at level 50).
+Notation "[ Γ ||-Id< l > t : A | RA ]" := (IdRedTmEq (Γ:=Γ) (l:=l) (A:=A) RA t t) (at level 0, Γ, l, t, A, RA at level 50).
+Notation "[ Γ ||-Id< l > t ≅ u : A | RA ]" := (IdRedTmEq (Γ:=Γ) (l:=l) (A:=A) RA t u) (at level 0, Γ, l, t, u, A, RA at level 50).
+
+
+
+
+
+
+
+
+
+
