theories/LogicalRelation/Definition/Nat.v
@@ -1,0 +1,150 @@
+(** * LogRel.LogicalRelation.Definition.Nat : Definition of the logical relation for TODO *)
+From Coq Require Import CRelationClasses.
+From LogRel Require Import Utils Syntax.All GenericTyping.
+From LogRel.LogicalRelation.Definition Require Import Prelude Ne.
+
+Set Primitive Projections.
+Set Universe Polymorphism.
+Set Polymorphic Inductive Cumulativity.
+
+
+(** ** Reducibility of natural number type *)
+Module NatRedTy.
+
+  Record NatRedTy `{ta : tag} `{WfType ta} `{RedType ta}
+    {Γ : context} {A B : term}
+  : Set :=
+  {
+    redL : [Γ |- A :⤳*: tNat] ;
+    redR : [Γ |- B :⤳*: tNat]
+  }.
+
+  Arguments NatRedTy {_ _ _}.
+
+  Section NatRedTy.
+  Context `{ta : tag} `{WfType ta} `{RedType ta}.
+
+  Definition whredL {Γ A B} : NatRedTy Γ A B -> [Γ |- A ↘].
+  Proof. intros []; econstructor; tea; constructor. Defined.
+
+  Definition whredR {Γ A B} : NatRedTy Γ A B -> [Γ |- B ↘].
+  Proof. intros []; econstructor; tea; constructor. Defined.
+
+  End NatRedTy.
+
+End NatRedTy.
+
+Export NatRedTy(NatRedTy, Build_NatRedTy).
+Notation "[ Γ ||-Nat A ≅ B ]" := (NatRedTy Γ A B) (at level 0, Γ, A at level 50).
+
+
+Module NatRedTmEq.
+Section NatRedTmEq.
+  Context `{ta : tag} `{WfContext ta} `{WfType ta} `{ConvType ta}
+    `{RedType ta} `{Typing ta} `{ConvNeuConv ta} `{ConvTerm ta}
+    `{RedTerm ta} {Γ : context}.
+
+  Inductive NatRedTmEq : term -> term -> Set :=
+  | Build_NatRedTmEq {t u}
+    (nfL nfR : term)
+    (redL : [Γ |- t :⤳*: nfL : tNat])
+    (redR : [Γ |- u :⤳*: nfR : tNat ])
+    (eq : [Γ |- nfL ≅ nfR : tNat])
+    (prop : NatPropEq nfL nfR) : NatRedTmEq t u
+
+  with NatPropEq : term -> term -> Set :=
+  | zeroReq :
+    NatPropEq tZero tZero
+  | succReq {n n'} :
+    NatRedTmEq n n' ->
+    NatPropEq (tSucc n) (tSucc n')
+  | neReq {ne ne'} : [Γ ||-NeNf ne ≅ ne' : tNat] -> NatPropEq ne ne'.
+
+  Section Def.
+    Context `{!GenericTypingProperties _ _ _ _ _ _ _ _ _ _ _ }.
+
+    Definition whnfL {t u} : NatPropEq t u -> whnf t.
+    Proof.
+      intros [].
+      1,2: constructor.
+      unshelve eapply NeNf.whredL; cycle 3; tea.
+    Qed.
+
+    Definition whnfR {t u} : NatPropEq t u -> whnf u.
+    Proof.
+      intros [].
+      1,2: constructor.
+      unshelve eapply NeNf.whredR; cycle 3; tea.
+    Qed.
+
+    Definition whredL {t u} : NatRedTmEq t u -> [Γ |- t ↘ tNat].
+    Proof.
+      intros []; econstructor; tea; now eapply whnfL.
+    Defined.
+
+    Definition whredR {t u} : NatRedTmEq t u -> [Γ |- u ↘ tNat].
+    Proof.
+      intros []; econstructor; tea; now eapply whnfR.
+    Defined.
+
+  End Def.
+
+(* Probably not useful anymore *)
+(*
+Definition nfL {Γ A B n m} {NA : [Γ ||-Nat A ≅ B]} : NatRedTmEq (NA:=NA) n m -> term.
+Proof.
+  intros [?? nf]. exact nf.
+Defined.
+
+Definition nfR {Γ A B n m} {NA : [Γ ||-Nat A ≅ B]} : NatRedTmEq (NA:=NA) n m -> term.
+Proof.
+  intros [?? ? nf]. exact nf.
+Defined.
+
+ Definition redL {Γ A n m} {NA : [Γ ||-Nat A]} (Rnm : NatRedTmEq (NA:=NA) n m) : [Γ |- n :⤳*: nfL Rnm : tNat].
+Proof.
+  dependent inversion Rnm; subst; cbn; tea.
+Defined.
+
+Definition redR {Γ A n m} {NA : [Γ ||-Nat A]} (Rnm : NatRedTmEq (NA:=NA) n m) : [Γ |- m :⤳*: nfR Rnm : tNat].
+Proof.
+  dependent inversion Rnm; subst; cbn; tea.
+Defined. *)
+
+Scheme NatRedTmEq_mut_rect := Induction for NatRedTmEq Sort Type with
+    NatPropEq_mut_rect := Induction for NatPropEq Sort Type.
+
+Combined Scheme _NatRedInduction from
+  NatRedTmEq_mut_rect,
+  NatPropEq_mut_rect.
+
+Combined Scheme _NatRedEqInduction from
+  NatRedTmEq_mut_rect,
+  NatPropEq_mut_rect.
+
+Let _NatRedEqInductionType :=
+  ltac:(let ind := fresh "ind" in
+      pose (ind := _NatRedEqInduction);
+      let ind_ty := type of ind in
+      exact ind_ty).
+
+Let NatRedEqInductionType :=
+  ltac: (let ind := eval cbv delta [_NatRedEqInductionType] zeta
+    in _NatRedEqInductionType in
+    let ind' := polymorphise ind in
+  exact ind').
+
+(* KM: looks like there is a bunch of polymorphic universes appearing there... *)
+Lemma NatRedEqInduction : NatRedEqInductionType.
+Proof.
+  intros PRedEq PPropEq **; split; now apply (_NatRedEqInduction PRedEq PPropEq).
+Defined.
+
+End NatRedTmEq.
+Arguments NatRedTmEq {_ _ _ _ _}.
+Arguments NatPropEq {_ _ _ _ _}.
+End NatRedTmEq.
+
+Export NatRedTmEq(NatRedTmEq,Build_NatRedTmEq, NatPropEq, NatRedEqInduction).
+
+Notation "[ Γ ||-Nat t ≅ u :Nat]" := (@NatRedTmEq _ _ _ _ _ _ _ Γ t u).  (* (at level 0, Γ, t, u, A, RA at level 50). *)
