theories/LogicalRelation/Definition/Ne.v
@@ -1,0 +1,103 @@
+(** * LogRel.LogicalRelation.Definition.Ne : Definition of the logical relation for neutal types and terms *)
+From Coq Require Import CRelationClasses.
+From LogRel Require Import Utils Syntax.All GenericTyping.
+From LogRel.LogicalRelation.Definition Require Import Prelude.
+
+Set Primitive Projections.
+Set Universe Polymorphism.
+Set Polymorphic Inductive Cumulativity.
+
+(** ** Reducibility of neutral types *)
+
+Module neRedTy.
+
+  Record neRedTy `{ta : tag}
+    `{WfType ta} `{ConvNeuConv ta} `{RedType ta}
+    {Γ : context} {A B : term}
+  : Set := {
+    tyL : term;
+    redL : [ Γ |- A :⤳*: tyL];
+    tyR : term;
+    redR : [ Γ |- B :⤳*: tyR];
+    eq : [ Γ |- tyL ~ tyR : U] ;
+  }.
+
+  Arguments neRedTy {_ _ _ _}.
+
+  Definition whredL `{GenericTypingProperties} {Γ : context} {A B : term} :
+    neRedTy Γ A B -> [Γ |- A ↘ ].
+  Proof. intros []; econstructor; tea; constructor; now eapply convneu_whne. Defined.
+
+  Definition whredR `{GenericTypingProperties} {Γ : context} {A B : term} :
+    neRedTy Γ A B -> [Γ |- B ↘ ].
+  Proof. intros []; econstructor; tea; constructor; eapply convneu_whne; now symmetry. Defined.
+
+End neRedTy.
+
+Export neRedTy(neRedTy, Build_neRedTy).
+Notation "[ Γ ||-ne A ≅ B ]" := (neRedTy Γ A B).
+
+
+Module neRedTmEq.
+
+  Record neRedTmEq `{ta : tag}
+    `{WfType ta} `{RedType ta}
+    `{Typing ta} `{ConvType ta} `{ConvTerm ta} `{ConvNeuConv ta} `{RedTerm ta}
+    {Γ : context} {t u A B : term} {R : [ Γ ||-ne A ≅ B]}
+  : Set := {
+    termL     : term;
+    termR     : term;
+    redL      : [ Γ |- t :⤳*: termL : R.(neRedTy.tyL) ];
+    redR      : [ Γ |- u :⤳*: termR : R.(neRedTy.tyL) ];
+    eq : [ Γ |- termL ~ termR : R.(neRedTy.tyL)] ;
+  }.
+
+  Arguments neRedTmEq {_ _ _ _ _ _ _ _ _} _ _ {_ _} _.
+
+  Definition whredL `{GenericTypingProperties} {Γ : context} {t u A B : term} {R : [ Γ ||-ne A ≅ B]} :
+    neRedTmEq t u R -> [Γ |- t ↘  R.(neRedTy.tyL)].
+  Proof.  intros []; econstructor; tea; constructor; now eapply convneu_whne. Defined.
+
+  Definition whredR `{GenericTypingProperties} {Γ : context} {t u A B : term} {R : [ Γ ||-ne A ≅ B]} :
+    neRedTmEq t u R -> [Γ |- u ↘  R.(neRedTy.tyL)].
+  Proof. intros []; econstructor; tea; constructor; eapply convneu_whne; now symmetry. Defined.
+
+End neRedTmEq.
+
+Export neRedTmEq(neRedTmEq, Build_neRedTmEq).
+Notation "[ Γ ||-ne t ≅ u : A | R ] " := (neRedTmEq (Γ:=Γ) (A:=A) t u R).
+
+
+(** ** Reducibility of neutrals at an arbitrary type *)
+
+Module NeNf.
+
+  Record RedTmEq `{ta : tag} `{Typing ta} `{ConvNeuConv ta} {Γ k l A} : Set :=
+    {
+      tyL : [Γ |- k : A] ;
+      tyR : [Γ |- l : A] ;
+      conv : [Γ |- k ~ l : A]
+    }.
+
+  Arguments RedTmEq {_ _ _}.
+
+  Definition whredL `{GenericTypingProperties} {Γ : context} {t u A : term} :
+    RedTmEq Γ t u A -> [Γ |- t ↘  A].
+  Proof.
+    intros []; econstructor.
+    1: now eapply redtmwf_refl.
+    constructor; now eapply convneu_whne.
+  Defined.
+
+  Definition whredR `{GenericTypingProperties} {Γ : context} {t u A : term} :
+    RedTmEq Γ t u A -> [Γ |- u ↘  A].
+  Proof.
+    intros []; econstructor.
+    1: now eapply redtmwf_refl.
+    constructor; eapply convneu_whne; now symmetry.
+  Defined.
+
+End NeNf.
+
+Notation "[ Γ ||-NeNf k ≅ l : A ]" := (NeNf.RedTmEq Γ k l A) (at level 0, Γ, k, l, A at level 50).
+
