theories/LogicalRelation/Definition/Pi.v
@@ -1,0 +1,104 @@
+(** * LogRel.LogicalRelation.Definition.Pi : Definition of the logical relation for dependent products *)
+From Coq Require Import CRelationClasses.
+From LogRel Require Import Utils Syntax.All GenericTyping.
+From LogRel.LogicalRelation.Definition Require Import Prelude Poly.
+
+Set Primitive Projections.
+Set Universe Polymorphism.
+Set Polymorphic Inductive Cumulativity.
+
+
+(** ** Reducibility of product types *)
+
+Definition PiRedTyPack `{ta : tag} `{WfContext ta} `{WfType ta} `{ConvType ta} `{RedType ta} :=
+  ParamRedTyPack (T:=tProd).
+
+Definition PiRedTyAdequate@{i j} `{ta : tag} `{WfContext ta} `{WfType ta} `{ConvType ta} `{RedType ta}
+    {Γ : context} {A B : term} (R : RedRel@{i j}) (ΠA : PiRedTyPack@{i} Γ A B)
+  : Type@{j} := PolyRedPackAdequate R ΠA.
+
+Module PiRedTyPack := ParamRedTyPack.
+
+Inductive isLRFun `{ta : tag} `{WfContext ta}
+  `{WfType ta} `{ConvType ta} `{RedType ta} `{Typing ta} `{ConvTerm ta} `{ConvNeuConv ta}
+  {Γ : context} {A B : term} (ΠA : PiRedTyPack Γ A B) : term -> Type :=
+| LamLRFun : forall A' t : term,
+    [Γ |- A'] ->
+    [Γ |-  ΠA.(PiRedTyPack.domL) ≅ A'] ->
+  (* (forall {Δ} (ρ : Δ ≤ Γ) (h : [ |- Δ ]) (domRed:= ΠA.(PolyRedPack.shpRed) ρ h),
+      [domRed | Δ ||- (PiRedTy.dom ΠA)⟨ρ⟩ ≅ A'⟨ρ⟩]) -> *)
+  (forall {Δ a b} (ρ : Δ ≤ Γ) (h : [ |- Δ ])
+    (ha : [ ΠA.(PolyRedPack.shpRed) ρ h | Δ ||- a ≅ b : ΠA.(PiRedTyPack.domL)⟨ρ⟩ ]),
+      [ΠA.(PolyRedPack.posRed) ρ h ha | Δ ||- t[a .: (ρ >> tRel)] ≅ t[b .: (ρ >> tRel)] : ΠA.(PiRedTyPack.codL)[a .: (ρ >> tRel)]]) ->
+  isLRFun ΠA (tLambda A' t)
+| NeLRFun : forall f : term, [Γ |- f ~ f : PiRedTyPack.outTy ΠA] -> isLRFun ΠA f.
+
+Module PiRedTmEq.
+
+  Import PiRedTyPack.
+
+  Definition appRed `{ta : tag} `{WfContext ta} `{WfType ta} `{ConvType ta} `{RedType ta}
+    {Γ A B} (ΠA : PiRedTyPack Γ A B) (nfL nfR : term) Δ a b :=
+    forall (ρ : Δ ≤ Γ) (h : [ |- Δ ])
+      (hab : [ΠA.(PolyRedPack.shpRed) ρ h | Δ ||- a ≅ b : ΠA.(domL)⟨ρ⟩ ] ),
+      [ ΠA.(PolyRedPack.posRed) ρ h hab | Δ ||- tApp nfL⟨ρ⟩ a ≅ tApp nfR⟨ρ⟩ b : _ ].
+
+  Arguments appRed /.
+
+  Record PiRedTm `{ta : tag} `{WfContext ta}
+    `{WfType ta} `{ConvType ta} `{RedType ta}
+    `{Typing ta} `{ConvTerm ta} `{ConvNeuConv ta} `{RedTerm ta}
+    {Γ : context} {A B} {ΠA : PiRedTyPack Γ A B} {t : term}
+  : Type := {
+    nf : term;
+    red : [ Γ |- t :⤳*: nf : outTy ΠA ];
+    isfun : isLRFun ΠA nf;
+    (* app {Δ a b} : appRed ΠA nf nf Δ a b; *)
+  }.
+
+  Arguments PiRedTm {_ _ _ _ _ _ _ _ _ _ _ _}.
+
+  Definition whred `{GenericTypingProperties}
+    {Γ : context} {A B} {ΠA : PiRedTyPack Γ A B} {t : term} :
+    PiRedTm ΠA t -> [Γ |- t ↘  outTy ΠA].
+  Proof.
+    intros [?? isfun]; econstructor; tea; destruct isfun.
+    1: gtyping.
+    constructor; now eapply convneu_whne.
+  Defined.
+
+  (* Lemma whnf `{GenericTypingProperties} {Γ A B} {ΠA : PiRedTy Γ A B} {t} : forall (red : PiRedTm ΠA t),
+    whnf (nf red).
+  Proof.
+    intros [? ? isfun]; simpl; destruct isfun; constructor; tea.
+    now eapply convneu_whne.
+  Qed. *)
+
+  Record PiRedTmEq `{ta : tag} `{WfContext ta}
+    `{WfType ta} `{ConvType ta} `{RedType ta}
+    `{Typing ta} `{ConvTerm ta} `{ConvNeuConv ta} `{RedTerm ta}
+    {Γ : context} {A B : term} {ΠA : PiRedTyPack Γ A B} {t u : term}
+  : Type := {
+    redL : PiRedTm ΠA t ;
+    redR : PiRedTm ΠA u ;
+    eq : [ Γ |- redL.(nf) ≅ redR.(nf) : outTy ΠA ];
+    eqApp {Δ a b} : appRed ΠA redL.(nf) redR.(nf) Δ a b;
+  }.
+
+  Arguments PiRedTmEq {_ _ _ _ _ _ _ _ _ _ _ _} _ _ _.
+
+  Definition whredL `{GenericTypingProperties}
+    {Γ : context} {A B} {ΠA : PiRedTyPack Γ A B} {t u : term} :
+    PiRedTmEq ΠA t u -> [Γ |- t ↘  outTy ΠA].
+  Proof. intros []; now eapply whred. Qed.
+
+  Definition whredR `{GenericTypingProperties}
+    {Γ : context} {A B} {ΠA : PiRedTyPack Γ A B} {t u : term} :
+    PiRedTmEq ΠA t u -> [Γ |- t ↘  outTy ΠA].
+  Proof. intros []; now eapply whred. Qed.
+
+End PiRedTmEq.
+
+Export PiRedTmEq(PiRedTm,Build_PiRedTm,PiRedTmEq,Build_PiRedTmEq).
+
+
