theories/LogicalRelation/Definition/Prelude.v
@@ -1,0 +1,85 @@
+(** * LogRel.LogicalRelation.Definition.Prelude: Structures employed to define the logical relation *)
+From Coq Require Import CRelationClasses.
+From LogRel Require Import Utils Syntax.All GenericTyping.
+
+Set Primitive Projections.
+Set Universe Polymorphism.
+Set Polymorphic Inductive Cumulativity.
+
+Create HintDb logrel.
+#[global] Hint Constants Opaque : logrel.
+#[global] Hint Variables Transparent : logrel.
+Ltac logrel := eauto with logrel.
+
+(** Note: modules are used as a hackish solution to provide a form of namespaces for record projections. *)
+
+(** ** Preliminaries *)
+
+(** Instead of using induction-recursion, we encode simultaneously the fact that a type is reducible,
+  and the graph of its decoding, as a single inductive relation.
+  Concretely, the type of our reducibility relation is the following RedRel:
+  for some R : RedRel, R Γ A eqTy redTm eqTm says
+  that according to R, A is reducible in Γ and the associated reducible type equality
+  (resp. term reducibility, term reducible equality) are eqTy (resp. redTm eqTm).
+  One should think of RedRel as a functional relation taking two arguments (Γ and A) and returning
+  three outputs (eqTy, redTm and eqTm). *)
+
+  Definition RedRel@{i j} :=
+  context               ->
+  term                  ->
+  term                  ->
+  (term -> term -> Type@{i}) ->
+  Type@{j}.
+
+(** An LRPack contains the data corresponding to the codomain of RedRel seen as a functional relation. *)
+
+Module LRPack.
+
+  Record LRPack@{i} {Γ : context} {A B : term} :=
+  {
+    eqTm :  term -> term -> Type@{i};
+  }.
+
+  Arguments LRPack : clear implicits.
+
+End LRPack.
+
+Export LRPack(LRPack,Build_LRPack).
+
+(* Notation "[ P | Γ ||- A ≅ B ]" := (@LRPack.eqTy Γ A P B). *)
+Notation "[ P | Γ ||- t : A ]" := (@LRPack.eqTm Γ A A P t t).
+Notation "[ P | Γ ||- t ≅ u : A ]" := (@LRPack.eqTm Γ A _ P t u).
+Notation "[ P | Γ ||- t ≅ u : A ≅ B ]" := (@LRPack.eqTm Γ A B P t u).
+
+(** An LRPack is adequate wrt. a RedRel when its three unpacked components are. *)
+Definition LRPackAdequate@{i j} {Γ : context} {A B : term}
+  (R : RedRel@{i j}) (P : LRPack@{i} Γ A B) : Type@{j} :=
+  R Γ A B P.(LRPack.eqTm).
+
+Arguments LRPackAdequate _ _ _ /.
+
+Module LRAd.
+
+  Record > LRAdequate@{i j} {Γ : context} {A B : term} {R : RedRel@{i j}} : Type :=
+  {
+    pack :> LRPack@{i} Γ A B ;
+    adequate :> LRPackAdequate@{i j} R pack
+  }.
+
+  Arguments LRAdequate : clear implicits.
+  Arguments Build_LRAdequate {_ _ _ _ _}.
+
+End LRAd.
+
+Export LRAd(LRAdequate,Build_LRAdequate).
+(* These coercions would be defined using the >/:> syntax in the definition of the record,
+  but this fails here due to the module being only partially exported *)
+Coercion LRAd.pack : LRAdequate >-> LRPack.
+Coercion LRAd.adequate : LRAdequate >-> LRPackAdequate.
+
+(* TODO : update these for LRAdequate *)
+
+Notation "[ R | Γ ||- A ≅ B ]"              := (@LRAdequate Γ A B R).
+(* Notation "[ R | Γ ||- A ≅ B | RA ]"     := (RA.(@LRAd.pack Γ A R).(LRPack.eqTy) B). *)
+Notation "[ R | Γ ||- t ≅ u : A | RA ]" := (RA.(@LRAd.pack Γ A _ R).(LRPack.eqTm) t u).
+Notation "[ R | Γ ||- t ≅ u : A ≅ B | RA ]" := (RA.(@LRAd.pack Γ A B R).(LRPack.eqTm) t u).
