theories/LogicalRelation/Definition/Universe.v
@@ -1,0 +1,118 @@
+(** * LogRel.LogicalRelation.Definition.Universe : Definition of the logical relation for universes *)
+From Coq Require Import CRelationClasses.
+From LogRel Require Import Utils Syntax.All GenericTyping.
+From LogRel.LogicalRelation.Definition Require Import Prelude.
+
+Set Primitive Projections.
+Set Universe Polymorphism.
+Set Polymorphic Inductive Cumulativity.
+
+
+(** ** Universe levels *)
+
+Inductive TypeLevel : Set :=
+  | zero : TypeLevel
+  | one  : TypeLevel.
+
+Inductive TypeLevelLt : TypeLevel -> TypeLevel -> Set :=
+    | Oi : TypeLevelLt zero one.
+
+Notation "A << B" := (TypeLevelLt A B).
+
+Definition LtSubst {l} (h : l = one) : zero << l.
+Proof.
+  rewrite h.
+  constructor.
+Qed.
+
+Definition elim {l : TypeLevel} (h : l << zero) : False :=
+  match h in _ << lz return (match lz with | zero => False | one => True end) with
+    | Oi => I
+  end.
+
+
+(** ** Reducibility of the universe *)
+
+Module URedTy.
+
+  Record URedTy `{ta : tag} `{!WfType ta} `{!RedType ta} `{H : WfContext ta} {l} {Γ : context} {A B : term}
+  : Set := {
+    level  : TypeLevel;
+    lt  : level << l;
+    redL : [ Γ |- A  :⤳*: U ] ;
+    redR : [ Γ |- B  :⤳*: U ] ;
+  }.
+
+  Arguments URedTy {_ _ _ _}.
+
+  Definition wfCtx  `{WfContextProperties}  {l} {Γ : context} {A B : term} : URedTy l Γ A B -> [|- Γ].
+  Proof. intros []; timeout 1 gen_typing. Qed.
+
+  Definition whredL `{ta : tag} `{!WfType ta} `{!RedType ta} `{WfContext ta} {l} {Γ : context} {A B : term} :
+    URedTy l Γ A B -> [Γ |- A ↘ ].
+  Proof. intros []; timeout 1 gen_typing. Defined.
+
+  Definition whredR `{ta : tag} `{!WfType ta} `{!RedType ta} `{WfContext ta} {l} {Γ : context} {A B : term} :
+    URedTy l Γ A B -> [Γ |- B ↘ ].
+  Proof. intros []; timeout 1 gen_typing. Defined.
+
+End URedTy.
+
+Export URedTy(URedTy,Build_URedTy).
+
+
+Notation "[ Γ ||-U< l > A ≅ B ]" := (URedTy l Γ A B) (at level 0, Γ, l, A, B at level 50).
+
+Module URedTm.
+
+  Record URedTm@{i j} `{ta : tag} `{WfContext ta} `{WfType ta}
+    `{Typing ta} `{ConvTerm ta} `{RedType ta} `{RedTerm ta}
+    {l} {rec : forall {l'}, l' << l -> RedRel@{i j}}
+    {Γ : context} {t A B : term} {R : [Γ ||-U<l> A ≅ B]}
+  : Type@{j} := {
+    te : term;
+    red : [ Γ |- t :⤳*: te : U ];
+    type : isType te;
+  }.
+
+  Arguments URedTm {_ _ _ _ _ _ _ _} rec.
+
+  Definition whred `{ta : tag} `{WfContext ta} `{WfType ta}
+    `{Typing ta} `{ConvTerm ta} `{RedType ta} `{RedTerm ta}
+    {l} {rec : forall l', l' << l -> RedRel}
+    {Γ : context} {t A B : term} {R : [Γ ||-U<l> A ≅ B]} :
+    URedTm rec Γ t A B R -> [Γ |- t ↘  U].
+  Proof. intros []; gtyping. Defined.
+
+  Record URedTmEq@{i j} `{ta : tag} `{WfContext ta} `{WfType ta}
+    `{Typing ta} `{ConvTerm ta} `{RedType ta} `{RedTerm ta}
+    {l} {rec : forall {l'}, l' << l -> RedRel@{i j}}
+    {Γ : context} {t u A B : term} {R : [Γ ||-U<l> A ≅ B]}
+  : Type@{j} := {
+      redL : URedTm (@rec) Γ t A B R ;
+      redR : URedTm (@rec) Γ u A B R ;
+      eq   : [ Γ |- redL.(te) ≅ redR.(te) : U ];
+      (* relEq : [ rec R.(URedTy.lt) | Γ ||- t ≅ u ] ; *)
+  }.
+
+  Arguments URedTmEq {_ _ _ _ _ _ _ _} rec.
+
+  Definition whredL `{ta : tag} `{WfContext ta} `{WfType ta}
+    `{Typing ta} `{ConvTerm ta} `{RedType ta} `{RedTerm ta}
+    {l} {rec : forall l', l' << l -> RedRel}
+    {Γ : context} {t u A B : term} {R : [Γ ||-U<l> A ≅ B]} :
+    URedTmEq rec Γ t u A B R -> [Γ |- t ↘  U].
+  Proof. intros []; now eapply whred. Defined.
+
+  Definition whredR `{ta : tag} `{WfContext ta} `{WfType ta}
+    `{Typing ta} `{ConvTerm ta} `{RedType ta} `{RedTerm ta}
+    {l} {rec : forall l', l' << l -> RedRel}
+    {Γ : context} {t u A B : term} {R : [Γ ||-U<l> A ≅ B]} :
+    URedTmEq rec Γ t u A B R -> [Γ |- u ↘  U].
+  Proof. intros []; now eapply whred. Defined.
+
+End URedTm.
+
+Export URedTm(URedTm,Build_URedTm,URedTmEq,Build_URedTmEq).
+Notation "[ R | Γ ||-U t ≅ u : A | l ]" := (URedTmEq R Γ t u A _ l) (at level 0, R, Γ, t, u, A, l at level 50).
+Notation "[ R | Γ ||-U t ≅ u : A ≅ B | l ]" := (URedTmEq R Γ t u A B l) (at level 0, R, Γ, t, u, A, B, l at level 50).
